

Perturbation Theory

Consider Hamiltonian of the following form

$$\hat{H}(t) = \hat{H}^{(0)} + \hat{H}^{(1)}(t), \quad (1)$$

where $\hat{H}^{(0)}$ is time-independent and is regarded as being solved with a full set of (eigenvalue, eigenstate) pairs

$$\hat{H}^{(0)} |\psi_n^{(0)}\rangle = \epsilon_n^{(0)} |\psi_n^{(0)}\rangle, \quad (2)$$

and $||\hat{H}^{(1)}|| \ll \delta\epsilon^{(0)}$ with $\delta\epsilon^{(0)}$ being the energy level spacing of the unperturbed spectrum¹. To keep track of the order of the corrections due to $\hat{H}^{(1)}$, we rewrite Eq. (1) as

$$\hat{H}(t, \lambda) = \hat{H}^{(0)} + \lambda \hat{H}^{(1)}(t), \quad (3)$$

and later use λ as an expansion parameter.

Our goal is to find, up to the j -th order correction in λ :

- when $\hat{H}^{(1)}$ is *time-independent*, the (eigenvalue, eigenstate) pairs of the full Hamiltonian:

$$\hat{H}(\lambda) |\psi_n(\lambda)\rangle = \epsilon_n(\lambda) |\psi_n(\lambda)\rangle \quad (4)$$

(λ is set to 1 at the end);

- when $\hat{H}^{(1)}(t)$ is *time-dependent*, the transition probability between unperturbed eigenstates $p_{m \leftarrow n}(t) \equiv \left| \left\langle \psi_m^{(0)} \right| \hat{U}(t, 0) \left| \psi_n^{(0)} \right\rangle \right|^2$.

¹The case of degenerate spectrum will be treated separately based on the nondegenerate solution.

1 Time-independent case

We start from formal expansions

$$\epsilon_n(\lambda) = \epsilon_n^{(0)} + \lambda \epsilon_n^{(2)} + \lambda^2 \epsilon_n^{(2)} + \dots, \quad (5)$$

$$|\psi_n(\lambda)\rangle = |\psi_n^{(0)}\rangle + \lambda |\psi_n^{(1)}\rangle + \lambda^2 |\psi_n^{(2)}\rangle + \dots, \quad (6)$$

where the above kets are not necessarily normalized (which does not affect the validity of Eq. (4)). We will fix, however, $|\psi_n^{(0)}\rangle$ to be always normalized such that $\langle \psi_m^{(0)} | \psi_n^{(0)} \rangle = \delta_{mn}$, and in addition $|\psi_n^{(j>0)}\rangle$ to be always orthogonal to $|\psi_n^{(0)}\rangle$ such that $\langle \psi_n^{(0)} | \psi_n^{(j>0)} \rangle = 0$. The latter condition can be seen as absorbing all possible $|\psi_n^{(0)}\rangle$ components in $|\psi_n^{(j>0)}\rangle$ into the zero-th order $|\psi_n^{(0)}\rangle$ (and then renormalize it). The normalization of $|\psi_n(\lambda)\rangle$ comes as the final step by taking $|\psi_n(\lambda)\rangle_{\text{normalized}} = |\psi_n(\lambda)\rangle / \sqrt{\langle \psi_n(\lambda) | \psi_n(\lambda) \rangle}$ and keeping the result up to $O(\lambda^j)$. For example,

$$\text{for } j = 1: \quad |\psi_n(\lambda)\rangle_{\text{normalized}} \simeq |\psi_n^{(0)}\rangle + \lambda |\psi_n^{(1)}\rangle; \quad (7)$$

$$\text{for } j = 2: \quad |\psi_n(\lambda)\rangle_{\text{normalized}} \simeq \left(1 - \frac{\lambda^2}{2} \langle \psi_n^{(1)} | \psi_n^{(1)} \rangle\right) |\psi_n^{(0)}\rangle + \lambda |\psi_n^{(1)}\rangle + \lambda^2 |\psi_n^{(2)}\rangle. \quad (8)$$

With the given problem, $\{|\psi_n^{(0)}\rangle\}$ is obviously “the” basis to work with. Let us use the un-hatted $H^{(0,1)}$ for the matrix representation of $\hat{H}^{(0,1)}$ in this basis:

$$H_{mn}^{(0,1)} = \langle \psi_m^{(0)} | \hat{H}^{(0,1)} | \psi_n^{(0)} \rangle, \quad (9)$$

and define matrices $E^{(j)}$ and $\Psi^{(j)}$ with their elements given by

$$E_{mn}^{(j)} = \epsilon_n^{(j)} \delta_{mn}, \quad \Psi_{mn}^{(j)} = \langle \psi_m^{(0)} | \psi_n^{(j)} \rangle. \quad (10)$$

Note that $E^{(j)}$ is always diagonal whereas $\Psi^{(j>0)}$ always has a vanishing diagonal.

It follows that Eq. (4) becomes

$$\begin{aligned} & (H^{(0)} + \lambda H^{(1)})(\Psi^{(0)} + \lambda \Psi^{(1)} + \lambda^2 \Psi^{(2)} + \dots) \\ &= (\Psi^{(0)} + \lambda \Psi^{(1)} + \lambda^2 \Psi^{(2)} + \dots)(E^{(0)} + \lambda E^{(1)} + \lambda^2 E^{(2)} + \dots), \end{aligned} \quad (11)$$

where, by construction,

$$H^{(0)} = E^{(0)}, \quad \Psi^{(0)} = \mathbb{1}. \quad (12)$$

Eq. (11) is the core of the time-independent perturbation theory. Let us break it down order by order:

$$\lambda^0 : \quad H^{(0)}\Psi^{(0)} = \Psi^{(0)}E^{(0)}; \quad (13)$$

$$\lambda^1 : \quad H^{(0)}\Psi^{(1)} + H^{(1)}\Psi^{(0)} = \Psi^{(0)}E^{(1)} + \Psi^{(1)}E^{(0)}; \quad (14)$$

$$\lambda^2 : \quad H^{(0)}\Psi^{(2)} + H^{(1)}\Psi^{(1)} = \Psi^{(0)}E^{(2)} + \Psi^{(1)}E^{(1)} + \Psi^{(2)}E^{(0)}; \quad (15)$$

$$\lambda^j : \quad H^{(0)}\Psi^{(j)} + H^{(1)}\Psi^{(j-1)} = \sum_{i=0}^j \Psi^{(i)}E^{(j-i)}. \quad (16)$$

As a consequence of the chosen basis, Eq. (13) is as trivial as $E^{(0)}\mathbb{1} = \mathbb{1}E^{(0)}$. Higher order equations become useful. Eq. (14) can be decoupled into diagonal and off-diagonal parts (note that $H^{(0)}\Psi^{(j>0)}$ and $\Psi^{(i>0)}E^{(i')}$ always have vanishing diagonals):

$$\text{diag}(H^{(1)}) = E^{(1)} \quad \text{or} \quad \epsilon_n^{(1)} = H_{nn}^{(1)}; \quad (17)$$

$$\text{offdiag}(E^{(0)}\Psi^{(1)} + H^{(1)}) = \text{offdiag}(\Psi^{(1)}E^{(0)}) \quad \text{or} \quad \Psi_{mn}^{(1)}|_{m \neq n} = -\frac{H_{mn}^{(1)}}{\epsilon_m^{(0)} - \epsilon_n^{(0)}}. \quad (18)$$

Similarly, Eq. (15) produces

$$\epsilon_n^{(2)} = \sum_{m \neq n} H_{nm}^{(1)}\Psi_{mn}^{(1)}; \quad (19)$$

$$\Psi_{mn}^{(2)}|_{m \neq n} = \frac{\Psi_{mn}^{(1)}H_{nn}^{(1)} - \sum_l H_{ml}^{(1)}\Psi_{ln}^{(1)}}{\epsilon_m^{(0)} - \epsilon_n^{(0)}}. \quad (20)$$

Or, generically,

$$\epsilon_n^{(j)} = (H^{(1)}\Psi^{(j-1)})_{nn} = \langle \psi_n^{(0)} | \hat{H}^{(1)} | \psi_n^{(j-1)} \rangle; \quad (21)$$

$$\Psi_{mn}^{(j)}|_{m \neq n} = \frac{(\sum_{i=1}^{j-1} \Psi^{(i)}E^{(j-i)} - H^{(1)}\Psi^{(j-1)})_{mn}}{\epsilon_m^{(0)} - \epsilon_n^{(0)}}. \quad (22)$$

The normalization of $\Psi = \sum_{i=0}^j \lambda^i \Psi^{(i)}$ is important but straightforward.

2 Time-dependent case

In this section, we shall write $\hat{V}(t) \equiv \hat{H}^{(1)}(t)$ and drop λ because the power of V already indicates the order of the correction. In the interaction picture, with the basis chosen to be $\{|\psi_n^{(0)}(t)\rangle\}$ with $|\psi_n^{(0)}(t)\rangle = \hat{U}^{(0)}(t)|\psi_n^{(0)}\rangle = \exp(-i\hat{H}^{(0)}t)|\psi_n^{(0)}\rangle = \exp(-i\epsilon_n^{(0)}t)|\psi_n^{(0)}\rangle$, a transition probability amplitudes can be identified (up to a phase factor) with a matrix elements of the interaction time-evolution operator

$$U^I(t)_{mn} = \langle \psi_m^{(0)} | \hat{U}^I(t) | \psi_n^{(0)} \rangle = \langle \psi_m^{(0)}(t) | \hat{U}(t) | \psi_n^{(0)} \rangle, \quad (23)$$

where

$$\frac{d}{dt}U^I(t) = -iV^I(t)U^I(t), \quad (24)$$

with

$$V_{mn}^I(t) = \langle \psi_m^{(0)}(t) | \hat{V}(t) | \psi_n^{(0)}(t) \rangle = V_{mn}(t)e^{i(\epsilon_m^{(0)} - \epsilon_n^{(0)})t}. \quad (25)$$

Eq. (24) is formally solved by the Dyson series

$$U^I(t) = 1 + (-i) \int_0^t dt_1 V^I(t_1) + (-i)^2 \int_0^t dt_1 V^I(t_1) \int_0^{t_1} dt_2 V^I(t_2) + \dots. \quad (26)$$

Eq. (26) is the core of the time-dependent perturbation theory.

To see it at work, let's study the example of the two-level (Rabi) model. In this case, $\epsilon_{\pm}^{(0)} = \pm\Omega/2$, and

$$V(t) = \begin{pmatrix} 0 & \gamma e^{-i\omega t} \\ \gamma e^{i\omega t} & 0 \end{pmatrix} \Rightarrow V^I(t) = \begin{pmatrix} 0 & \gamma e^{i(\Omega-\omega)t} \\ \gamma e^{-i(\Omega-\omega)t} & 0 \end{pmatrix}. \quad (27)$$

The first order term in Eq. (26) becomes

$$(-i) \int_0^t dt_1 V^I(t_1) = \begin{pmatrix} 0 & -\frac{\gamma}{\Omega-\omega} [e^{i(\Omega-\omega)t} - 1] \\ \frac{\gamma}{\Omega-\omega} [e^{-i(\Omega-\omega)t} - 1] & 0 \end{pmatrix}. \quad (28)$$

The second order term in Eq. (26) becomes

$$\begin{aligned} & (-i)^2 \int_0^t dt_1 V^I(t_1) \int_0^{t_1} dt_2 V^I(t_2) \\ &= \begin{pmatrix} -i\frac{\gamma^2}{\Omega-\omega}t + (\frac{\gamma}{\Omega-\omega})^2 [e^{i(\Omega-\omega)t} - 1] & 0 \\ 0 & i\frac{\gamma^2}{\Omega-\omega}t + (\frac{\gamma}{\Omega-\omega})^2 [e^{-i(\Omega-\omega)t} - 1] \end{pmatrix}. \end{aligned} \quad (29)$$

A Exact solution of the two-level model

In a pre-chosen basis, the model Hamiltonian reads

$$H = \begin{pmatrix} \Omega/2 & \gamma e^{-i\omega t} \\ \gamma e^{i\omega t} & -\Omega/2 \end{pmatrix} \quad (\Omega, \gamma, \omega \geq 0). \quad (30)$$

Let us define

$$\Delta \equiv \sqrt{(\Omega/2)^2 + \gamma^2}, \quad \cos \theta \equiv \frac{\Omega/2}{\Delta}, \quad \sin \theta \equiv \frac{\gamma}{\Delta}, \quad (31)$$

such that

$$H = \Delta \begin{pmatrix} \cos \theta & \sin \theta e^{-i\omega t} \\ \sin \theta e^{i\omega t} & -\cos \theta \end{pmatrix}. \quad (32)$$

When $\omega = 0$ (i.e. H is time-independent), the eigenvalues and the corresponding eigenstates are

$$\epsilon_{\pm} = \pm \Delta, \quad \psi_+ = \begin{pmatrix} \cos \frac{\theta}{2} \\ \sin \frac{\theta}{2} \end{pmatrix}, \quad \psi_- = \begin{pmatrix} \sin \frac{\theta}{2} \\ -\cos \frac{\theta}{2} \end{pmatrix}. \quad (33)$$

If $\gamma \ll \Omega$, we can expand, up to $(\gamma/\Omega)^2$,

$$\Delta \simeq (\Omega/2) \left[1 + \frac{1}{2} \left(\frac{\gamma}{\Omega/2} \right)^2 \right] \simeq \frac{\Omega}{2} + \frac{\gamma^2}{\Omega}, \quad (34)$$

$$\cos \frac{\theta}{2} = \sqrt{\frac{1}{2}(1 + \cos \theta)} = \sqrt{\frac{1}{2}(1 + \left[1 + \left(\frac{\gamma}{\Omega/2} \right)^2 \right]^{-1/2})} \simeq 1 - \frac{1}{2} \left(\frac{\gamma}{\Omega} \right)^2, \quad (35)$$

$$\sin \frac{\theta}{2} = \sqrt{\frac{1}{2}(1 - \cos \theta)} = \sqrt{\frac{1}{2}(1 - \left[1 + \left(\frac{\gamma}{\Omega/2} \right)^2 \right]^{-1/2})} \simeq \frac{\gamma}{\Omega}. \quad (36)$$

These expansions allow us to compare the exact solutions in Eq. (33) with a time-independent perturbation calculation.

When $\omega > 0$ (i.e. H is time-dependent), we aim to solve for the time-evolution operator $U(t) \equiv U(t, 0)$ which satisfies

$$\frac{d}{dt} U(t) = -iH(t)U(t). \quad (37)$$

We first transform

$$\tilde{H} = \rho_\omega(t)H(t)\rho_\omega(t)^{-1} = \begin{pmatrix} \Omega/2 & \gamma \\ \gamma & -\Omega/2 \end{pmatrix}, \quad (38)$$

$$\tilde{U}(t) = \rho_\omega(t)U(t), \quad (39)$$

where

$$\rho_\omega(t) \equiv \begin{pmatrix} e^{i\omega t/2} & \\ & e^{-i\omega t/2} \end{pmatrix}. \quad (40)$$

Then Eq. (37) becomes

$$\frac{d}{dt}\tilde{U}(t) = -i(\tilde{H} - \frac{\omega}{2}\sigma_z)\tilde{U}(t). \quad (41)$$

Now we have a time-independent “effective” Hamiltonian such that we immediately obtain

$$\tilde{U}(t) = \exp[-i(\tilde{H} - \frac{\omega}{2}\sigma_z)t] \quad (42)$$

$$= \cos(\Delta_\omega t) - i \sin(\Delta_\omega t)(\cos \theta_\omega \sigma_z + \sin \theta_\omega \sigma_x), \quad (43)$$

where

$$\Delta_\omega \equiv \sqrt{(\frac{\Omega - \omega}{2})^2 + \gamma^2}, \quad \cos \theta_\omega \equiv \frac{(\Omega - \omega)/2}{\Delta_\omega}, \quad \sin \theta_\omega \equiv \frac{\gamma}{\Delta_\omega}. \quad (44)$$

If the initial state at $t = 0$ is given by $\psi(0) = \begin{pmatrix} 1 \\ 0 \end{pmatrix}$, then

$$\psi(t) = U(t)\psi(0) = \begin{pmatrix} e^{-i\omega t/2}[\cos(\Delta_\omega t) - i \sin(\Delta_\omega t) \cos \theta_\omega] \\ -ie^{i\omega t/2} \sin(\Delta_\omega t) \sin \theta_\omega \end{pmatrix}. \quad (45)$$

It follows that the transition probability from the first component to the second is given by

$$p(t) = \sin^2(\Delta_\omega t) \sin^2 \theta_\omega = \frac{\gamma^2}{(\frac{\Omega - \omega}{2})^2 + \gamma^2} \sin^2(\Delta_\omega t). \quad (46)$$